code/ecdsa/Hacl.Impl.P256.Compression.fsti
@@ -16,25 +16,31 @@ open Spec.ECC.Curves
 open Hacl.Spec.MontgomeryMultiplication
 
 
-let notCompressedForm = lbuffer uint8 (size 65)
-let compressedForm = lbuffer uint8 (size 33)
+#set-options "--z3rlimit 200 --ifuel 0 --fuel 0" 
+
+
+let notCompressedForm (c: curve) = lbuffer uint8 (getCoordinateLenU c *! 2ul +! 1ul)
+
+let compressedForm (c: curve) = lbuffer uint8 (getCoordinateLenU c +! 1ul)
+
 
 inline_for_extraction
-val decompressionNotCompressedForm: #c: curve -> b: notCompressedForm -> result: lbuffer uint8 (size 64) -> Stack bool 
+val decompressionNotCompressedForm: #c: curve -> b: notCompressedForm c -> result: lbuffer uint8 (getCoordinateLenU c *! 2ul) -> Stack bool 
   (requires fun h -> live h b /\ live h result /\ disjoint b result)
-  (ensures fun h0 r h1 -> modifies (loc result) h0 h1 /\
-    (
-      let id = Lib.Sequence.index (as_seq h0 b) 0 in 
-      let x = Lib.Sequence.sub (as_seq h0 b) 1 32 in 
-	let xResult = Lib.Sequence.sub (as_seq h1 result) 0 32 in 
-      let y = Lib.Sequence.sub (as_seq h0 b) 33 32 in 
-	let yResult = Lib.Sequence.sub (as_seq h1 result) 32 32 in 
-	  if uint_v id = 4 then 
-	    r == true /\ x == xResult /\ y == yResult
-  	  else 
-	    r == false
-  	)
-)
+  (ensures fun h0 r h1 -> modifies (loc result) h0 h1 /\ (
+    let len = v (getCoordinateLenU c) in 
+    
+    let id = Lib.Sequence.index (as_seq h0 b) 0 in 
+    let x = Lib.Sequence.sub (as_seq h0 b) 1 len in 
+    let y = Lib.Sequence.sub (as_seq h0 b) (len + 1) len in 
+
+    let xResult = Lib.Sequence.sub (as_seq h1 result) 0 len in 
+    let yResult = Lib.Sequence.sub (as_seq h1 result) len len in 
+    if uint_v id = 4 then 
+       r == true /\ x == xResult /\ y == yResult
+    else 
+      r == false))
+
 
 inline_for_extraction
 val decompressionCompressedForm: #c: curve -> b: compressedForm -> result: lbuffer uint8 (size 64) -> Stack bool 
